Core/Process.v
@@ -15,15 +15,13 @@ Unset Printing Implicit Defensive.
 
 Section ProcessSyntax.
 
-Variable this : nid.
-
 (* Syntax for process *)
 Inductive proc (W : world) A :=
-  Unfinished | Ret of A | Act of action W A this |
+  Unfinished | Ret of A | Act (this : nid) of action W A this |
   Seq B of proc W B & B -> proc W A |
   Inject V K of injects V W K & proc V A |
   WithInv p I (ii : InductiveInv p I) of
-          W = mkWorld (ProtocolWithIndInv ii) & proc (mkWorld p) A.  
+          W = mkWorld (ProtocolWithIndInv ii) & proc (mkWorld p) A.
 
 Definition pcat W A B (t : proc W A) (k : A -> Pred (proc W B)) :=
   [Pred s | exists q, s = Seq t q /\ forall x, q x \In k x].
@@ -35,21 +33,19 @@ Inductive schedule :=
 
 End ProcessSyntax.
 
-Implicit Arguments Unfinished [this W A].
-Implicit Arguments Ret [this W A].
-Implicit Arguments Act [this W A].
-Implicit Arguments Seq [this W A B].
-Implicit Arguments WithInv [this W A].
+Implicit Arguments Unfinished [W A].
+Implicit Arguments Ret [W A].
+Implicit Arguments Act [W A].
+Implicit Arguments Seq [W A B].
+Implicit Arguments WithInv [W A].
 
 Section ProcessSemantics.
 
-Variable this : nid.
-
-Fixpoint step (W : world) A (s1 : state) (p1 : proc this W A)
-         sc (s2 : state) (p2 : proc this W A) : Prop :=
+Fixpoint step (W : world) A (s1 : state) (p1 : proc W A)
+         sc (s2 : state) (p2 : proc W A) : Prop :=
   match sc, p1 with
   (* Action - make a step *)  
-  | ActStep, Act a => exists v pf, @a_step _ _ _ a s1 pf s2 v /\ p2 = Ret v
+  | ActStep, Act this a => exists v pf, @a_step _ _ this a s1 pf s2 v /\ p2 = Ret v
   (* Sequencing - apply a continuation *)  
   | SeqRet, Seq _ (Ret v) k => s2 = s1 /\ p2 = k v
   | SeqStep sc', Seq _ p' k1 => 
@@ -70,9 +66,9 @@ Fixpoint step (W : world) A (s1 : state) (p1 : proc this W A)
   | _, _ => False
   end.
 
-Fixpoint good (W : world) A (p : proc this W A) sc  : Prop :=
+Fixpoint good (W : world) A (p : proc W A) sc  : Prop :=
   match sc, p with
-  | ActStep, Act _ => True
+  | ActStep, Act _ _ => True
   | SeqRet, Seq _ (Ret _) _ => True
   | SeqStep sc', Seq _ p' _ => good p' sc'
   | InjectStep sc', Inject _ _ _ p' => good p' sc'
@@ -94,28 +90,27 @@ structure. Once it's dropped, this structure is lost.
 
  *)
 
-Fixpoint safe (W : world) A (p : proc this W A) sc (s : state)  : Prop :=
+Fixpoint safe (W : world) A (p : proc W A) (this : nid) sc (s : state) : Prop :=
   match sc, p with
-  | ActStep, Act a => a_safe a s
+  | ActStep, Act n a => n == this /\ @a_safe _ _ n a s
   | SeqRet, Seq _ (Ret _) _ => True
-  | SeqStep sc', Seq _ p' _ => safe p' sc' s
+  | SeqStep sc', Seq _ p' _ => safe p' this sc' s
   | InjectStep sc', Inject V K pf p' =>
-      exists s', extends pf s s' /\ safe p' sc' s'
+      exists s', extends pf s s' /\ safe p' this sc' s'
   | InjectRet, Inject V K pf (Ret _) => exists s', extends pf s s'
-  | WithInvStep sc', WithInv _ _ _ _ p' => safe p' sc' s
+  | WithInvStep sc', WithInv _ _ _ _ p' => safe p' this sc' s
   | WithInvRet, WithInv _ _ _ _ (Ret _) => True
   | _, _ => True
   end.
 
-Definition pstep (W : world) A s1 (p1 : proc this W A) sc s2 p2 := 
-  [/\ s1 \In Coh W, safe p1 sc s1 & step s1 p1 sc s2 p2].
+Definition pstep (W : world) A s1 (p1 : proc W A) this sc s2 p2 := 
+  [/\ s1 \In Coh W, safe p1 this sc s1 & step s1 p1 sc s2 p2].
 
 (* Some sanity lemmas wrt. stepping *)
 
-Lemma pstep_safe (W : world) A s1 (t : proc this W A) sc s2 q : 
-        pstep s1 t sc s2 q -> safe t sc s1.
+Lemma pstep_safe (W : world) A s1 (t : proc W A) this sc s2 q : 
+        pstep s1 t this sc s2 q -> safe t this sc s1.
 Proof. by case. Qed.
-
 
 (*
 
@@ -124,27 +119,27 @@ program, which is safe and also the schedule is appropriate. Together,
 this implies that we can do a step. 
  *)
 
-Lemma proc_progress W A s (p : proc this W A) sc : 
-        s \In Coh W -> safe p sc s -> good p sc ->  
-        exists s' (p' : proc this W A), pstep s p sc s' p'.
+Lemma proc_progress W A s (p : proc W A) this sc : 
+        s \In Coh W -> safe p this sc s -> good p sc ->  
+        exists s' (p' : proc W A), pstep s p this sc s' p'.
 Proof.
-move=>C H1 H2; elim: sc W A s p H2 H1 C=>[||sc IH|sc IH||sc IH|]W A s. 
-- case=>//=a _/= H; move/a_step_total: (H)=>[s'][r]H'.
+move=>C H1 H2; elim: sc W A this s p H2 H1 C=>[||sc IH|sc IH||sc IH|]W A this s. 
+- case=>//=n a _/= [E H]; move/a_step_total: (H)=>[s'][r]H'.
   by exists s', (Ret r); split=>//=; exists r, H.  
 - by case=>//; move=>B p k/=; case: p=>//b _ _; exists s, (k b). 
 - case=>//B p k/=H1 H2 C.
-  case: (IH W B s p H1 H2 C)=>s'[p'][G1 G2].
+  case: (IH W B this s p H1 H2 C)=>s'[p'][G1 G2].
   by exists s', (Seq p' k); split=>//; exists p'. 
 - case=>// V K pf p/=H1 [z][E]H2 C. 
   case: (E)=>s3[Z] C1 C2.
-  case: (IH V A z p H1 H2 C1) =>s'[p']H3; case: H3=>S St.
+  case: (IH V A this z p H1 H2 C1) =>s'[p']H3; case: H3=>S St.
   exists (s' \+ s3), (Inject pf p'); split=>//; first by exists z.  
   by subst s; exists z, s', s3, p'. 
 - case=>//V K pf; case=>// v/=_[s'] E C.          
   by exists s, (Ret v); split=>//=; exists s'.
 - case=>//pr I ii E p/= H1 H2 C.
   have C' : s \In Coh (mkWorld pr) by subst W; apply: (with_inv_coh C). 
-  case: (IH (mkWorld pr) A s p H1 H2 C')=>s'[p']H3.
+  case: (IH (mkWorld pr) A this s p H1 H2 C')=>s'[p']H3.
   exists s', (WithInv pr I ii E p'); split=>//=.
   by exists p'; split=>//; case: H3. 
 - case=>//pr I ii E; case=>//v/=_ _ C.          
@@ -153,29 +148,29 @@ Qed.
 
 (* Some view lemmas for processes and corresponding schedules *)
 
-Lemma stepUnfin W A s1 sc s2 (t : proc this W A) : 
-        pstep s1 Unfinished sc s2 t <-> False.
+Lemma stepUnfin W A s1 this sc s2 (t : proc W A) : 
+        pstep s1 Unfinished this sc s2 t <-> False.
 Proof. by split=>//; case; case: sc. Qed.
 
-Lemma stepRet W A s1 sc s2 (t : proc this W A) v : 
-        pstep s1 (Ret v) sc s2 t <-> False.
+Lemma stepRet W A s1 this sc s2 (t : proc W A) v : 
+        pstep s1 (Ret v) this sc s2 t <-> False.
 Proof. by split=>//; case; case: sc. Qed.
 
-Lemma stepAct W A s1 a sc s2 (t : proc this W A) : 
-        pstep s1 (Act a) sc s2 t <->
-        exists v pf, [/\ sc = ActStep, t = Ret v & @a_step _ _ _ a s1 pf s2 v].
+Lemma stepAct W A s1 n this a sc s2 (t : proc W A) : 
+        pstep s1 (Act n a) this sc s2 t <->
+        exists v pf, [/\ sc = ActStep, t = Ret v, n == this & @a_step _ _ _ a s1 pf s2 v].
 Proof.
-split; first by case=>C; case: sc=>//= c [v [pf [H ->]]]; exists v, pf. 
+split; first by case=>C; case: sc=>//= [[G c]][v [pf [H ->]]]; exists v, pf. 
 case=>v[pf] [->-> H]; split=>//; last by exists v, pf.
 by apply: (a_safe_coh pf). 
 Qed.
 
-Lemma stepSeq W A B s1 (t : proc this W B) k sc s2 (q : proc this W A) :
-        pstep s1 (Seq t k) sc s2 q <->
+Lemma stepSeq W A B s1 (t : proc W B) k this sc s2 (q : proc W A) :
+        pstep s1 (Seq t k) this sc s2 q <->
         (exists v, [/\ sc = SeqRet, t = Ret v, q = k v, s2 = s1 &
                        s1 \In Coh W]) \/
          exists sc' p',
-           [/\ sc = SeqStep sc', q = Seq p' k & pstep s1 t sc' s2 p'].
+           [/\ sc = SeqStep sc', q = Seq p' k & pstep s1 t this sc' s2 p'].
 Proof.
 split; last first.
 - case; first by case=>v [->->->->]. 
@@ -186,8 +181,8 @@ by move=>G /= [p' [H1 ->]]; right; exists sc, p'.
 Qed.
 
 Lemma stepInject V W K A (em : injects V W K) 
-                s1 (t : proc this V A) sc s2 (q : proc this W A) :
-  pstep s1 (Inject em t) sc s2 q <->
+                s1 (t : proc V A) this sc s2 (q : proc W A) :
+  pstep s1 (Inject em t) this sc s2 q <->
   (* Case 1 : stepped to the final state s1' of the inner program*)
   (exists s1' v, [/\ sc = InjectRet, t = Ret v, q = Ret v, s2 = s1 &
                      extends em s1 s1']) \/
@@ -195,7 +190,7 @@ Lemma stepInject V W K A (em : injects V W K)
   exists sc' t' s1' s2' s, 
     [/\ sc = InjectStep sc', q = Inject em t', 
      s1 = s1' \+ s, s2 = s2' \+ s, s1 \In Coh W &
-              pstep s1' t sc' s2' t'].
+              pstep s1' t this sc' s2' t'].
 Proof.
 split; last first.
 - case.
@@ -213,13 +208,13 @@ by case: X=>t'' [E] Cs' _; rewrite (coh_prec (cohS C) E _ Cs').
 Qed.
 
 Lemma stepWithInv W A pr I (ii : InductiveInv pr I) s1 
-      (t : proc this (mkWorld pr) A) sc s2 (q : proc this W A) pf :
-  pstep s1 (WithInv pr I ii pf t) sc s2 q <-> 
+      (t : proc (mkWorld pr) A) this sc s2 (q : proc W A) pf :
+  pstep s1 (WithInv pr I ii pf t) this sc s2 q <-> 
   (exists v, [/\ sc = WithInvRet, t = Ret v, q = Ret v, s2 = s1,
                  s1 \In Coh W & W = mkWorld (ProtocolWithIndInv ii)]) \/
   exists sc' t' , [/\ sc = WithInvStep sc', q = WithInv pr I ii pf t',
                       W = mkWorld (ProtocolWithIndInv ii),
-                      s1 \In Coh W & pstep s1 t sc' s2 t'].
+                      s1 \In Coh W & pstep s1 t this sc' s2 t'].
 Proof.
 split; last first.
 - case.
@@ -240,26 +235,27 @@ programs respect the global network semantics.
 
  *)
 
-Lemma pstep_network_sem (W : world) A s1 (t : proc this W A) sc s2 q :
-        pstep s1 t sc s2 q -> network_step W this s1 s2.
+Lemma pstep_network_sem (W : world) A s1 (t : proc W A) this sc s2 q :
+        pstep s1 t this sc s2 q -> network_step W this s1 s2.
 Proof.
-elim: sc W A s1 s2 t q=>/=.
-- move=>W A s1 s2 p q; case: p; do?[by case|by move=>?; case].
-  + by move=>a/stepAct [v][pf][Z1]Z2 H; subst q; apply: (a_step_sem H).
+elim: sc W A this s1 s2 t q=>/=.
+- move=>W A this s1 s2 p q; case: p; do?[by case|by move=>?; case| by move=>??; case].
+  + move=>n a/stepAct[v][pf][Z1]Z2 /eqP Z H; subst n.
+    by subst q; apply: (a_step_sem H).
   + by move=>???; case. 
   + by move=>????; case.
   by move=>?????; case.   
-- move=>W A s1 s2 p q; case: p; do?[by case|by move=>?; case].
+- move=>W A this s1 s2 p q; case: p; do?[by case|by move=>?; case| by move=>??; case].
   + move=>B p p0/stepSeq; case=>[[v][_]??? C|[sc'][p'][]]//.
     by subst p s2; apply: Idle. 
   by move=>????/stepInject; case=>[[?][?][?]|[?][?][?][?][?][?]]//.
   by move=>?????; case.   
-- move=>sc HI W A s1 s2 p q; case: p; do?[by case|by move=>?; case].
+- move=>sc HI W A this s1 s2 p q; case: p; do?[by case|by move=>?; case| by move=>??; case].
   + move=>B p p0/stepSeq; case=>[[?][?]|[sc'][p'][][]? ?]//.
     by subst sc' q; apply: HI.
   by move=>????; case=>? _.
   by move=>?????; case.   
-- move=>sc HI W A s1 s2 p q; case: p; do?[by case|by move=>?; case].
+- move=>sc HI W A this s1 s2 p q; case: p; do?[by case|by move=>?; case| by move=>??; case].
   + by move=>B p p0; case. 
   move=>V K pf p/stepInject; case=>[[?][?][?]|[sc'][t'][s1'][s2'][s][][]????]//. 
   subst sc' q s1 s2=>C; move/HI=>S; apply: (sem_extend pf)=>//.
@@ -267,20 +263,20 @@ elim: sc W A s1 s2 t q=>/=.
   move/(cohE pf): (C)=>[s1][s2][E]C' H.
   by move: (coh_prec (cohS C) E C1 C')=>Z; subst s1'; rewrite (joinfK (cohS C) E). 
   by move=>?????; case.   
-- move=>W A s1 s2 p q; case: p; do?[by case|by move=>?; case].
+- move=>W A this s1 s2 p q; case: p; do?[by case|by move=>?; case| by move=>??; case].
   + by move=>???; case.
   + move=>V K i p; case/stepInject=>[[s1'][v][_]??? X|[?][?][?][?][?][?]]//.
     by subst p q s2; apply: Idle; split=>//; case: X=>x []. 
   by move=>?????; case.
-
-- move=>sc HI W A s1 s2 p q; case: p;
-           do?[by case|by move=>?; case|by move=>???; case|by move=>????; case].
+- move=>sc HI W A this s1 s2 p q; case: p;
+          do?[by case|by move=>?; case| by move=>??; case
+              |by move=>???; case|by move=>????; case].
   move=>pr I ii E p; case/(stepWithInv s1); first by case=>?; case.
   case=>sc'[t'][][]Z1 Z2 _ C1; subst q sc'.
   by move/HI=>T; subst W; apply: with_inv_step. 
-move=>W A s1 s2 t q; do?[by case|by move=>?; case|by move=>???; case].
-case=>C; case: t=>//pr I ii E; case=>//=v _[s1'][Z1]Z2 Z3.
-by subst s1' s2 q; apply: Idle. 
+- move=>W A this s1 s2 t q; do?[by case|by move=>?; case|by move=>???; case].
+  case=>C; case: t=>//pr I ii E; case=>//=v _[s1'][Z1]Z2 Z3.
+  by subst s1' s2 q; apply: Idle.
 Qed.
 
 (*
@@ -292,10 +288,10 @@ it leverages the proof of the fact that each transition preserves the invariant.
 
 *)
 
-Lemma pstep_inv A pr I (ii : InductiveInv pr I) s1 s2 sc
-      (t t' : proc this (mkWorld pr) A):
+Lemma pstep_inv A pr I (ii : InductiveInv pr I) s1 s2 this sc
+      (t t' : proc (mkWorld pr) A):
   s1 \In Coh (mkWorld (ProtocolWithIndInv ii)) ->
-  pstep s1 t sc s2 t' -> 
+  pstep s1 t this sc s2 t' -> 
   s2 \In Coh (mkWorld (ProtocolWithIndInv ii)).
 Proof. by move=>C1; case/pstep_network_sem/(with_inv_step C1)/step_coh. Qed.
 
