Core/Process1.v
@@ -1,0 +1,697 @@
+Require Import Relation_Operators.
+Require Import pred prelude idynamic ordtype finmap pcm unionmap heap coding.
+Require Import Freshness State EqTypeX DepMaps Protocols Worlds NetworkSem.
+Require Import Actions Injection.
+Require Import InductiveInv.
+
+Set Implicit Arguments.
+Unset Strict Implicit.
+Unset Printing Implicit Defensive.
+
+Section ProcessSyntax.
+
+(* Syntax for process *)
+Inductive proc (W : world) A :=
+  Unfinished | Ret of A | Act (this : nid) of action W A this |
+  Seq B of proc W B & B -> proc W A |
+  Inject V K of injects V W K & proc V A |
+  WithInv p I (ii : InductiveInv p I) of
+          W = mkWorld (ProtocolWithIndInv ii) & proc (mkWorld p) A |
+  (* Top-level parallel composition *)
+  ParProc of seq (nid * (proc W A)).
+
+Definition pcat W A B (t : proc W A) (k : A -> Pred (proc W B)) :=
+  [Pred s | exists q, s = Seq t q /\ forall x, q x \In k x].
+Require Import Relation_Operators.
+Require Import pred prelude idynamic ordtype finmap pcm unionmap heap coding.
+Require Import Freshness State EqTypeX DepMaps Protocols Worlds NetworkSem.
+Require Import Actions Injection.
+Require Import InductiveInv.
+
+Set Implicit Arguments.
+Unset Strict Implicit.
+Unset Printing Implicit Defensive.
+
+Section ProcessSyntax.
+
+(* Syntax for process *)
+Inductive proc (W : world) A :=
+  Unfinished | Ret of A | Act (this : nid) of action W A this |
+  Seq B of proc W B & B -> proc W A |
+  Inject V K of injects V W K & proc V A |
+  WithInv p I (ii : InductiveInv p I) of
+          W = mkWorld (ProtocolWithIndInv ii) & proc (mkWorld p) A |
+  (* Top-level parallel composition *)
+  ParProc of seq (nid * (proc W A)).
+
+Definition pcat W A B (t : proc W A) (k : A -> Pred (proc W B)) :=
+  [Pred s | exists q, s = Seq t q /\ forall x, q x \In k x].
+
+Inductive schedule :=
+  ActStep | SeqRet | SeqStep of schedule |  
+  InjectStep of schedule | InjectRet |
+  WithInvStep of schedule | WithInvRet |
+  (* Step node number n *)
+  ParStep (n : nid) of schedule.
+
+End ProcessSyntax.
+
+Implicit Arguments Unfinished [W A].
+Implicit Arguments Ret [W A].
+Implicit Arguments Act [W A].
+Implicit Arguments Seq [W A B].
+Implicit Arguments WithInv [W A].
+Implicit Arguments ParProc [W A].
+
+Section ProcessSemantics.
+
+Fixpoint step (W : world) A (s1 : state) (p1 : proc W A)
+         sc (s2 : state) (p2 : proc W A) : Prop :=
+  match sc, p1 with
+  (* Action - make a step *)  
+  | ActStep, Act this a => exists v pf, @a_step _ _ this a s1 pf s2 v /\ p2 = Ret v
+  (* Sequencing - apply a continuation *)  
+  | SeqRet, Seq _ (Ret v) k => s2 = s1 /\ p2 = k v
+  | SeqStep sc', Seq _ p' k1 => 
+    exists p'', step s1 p' sc' s2 p'' /\ p2 = Seq p'' k1
+  (* Injection of a non-reduced term *)
+  | InjectRet, Inject V K pf (Ret v) =>
+     exists s1', [/\ s2 = s1, p2 = Ret v & extends pf s1 s1']
+  | InjectStep sc', Inject V K pf t1' =>
+    exists s1' s2' s t2', 
+    [/\ p2 = Inject pf t2', s1 = s1' \+ s, s2 = s2' \+ s, 
+     s1' \In Coh V & step s1' t1' sc' s2' t2']
+  (* Imposing an inductive invariant on a non-reduced term *)
+  | WithInvRet, WithInv p inv ii pf (Ret v) =>
+     exists s1', [/\ s2 = s1, p2 = Ret v & s1 = s1']
+  | WithInvStep sc', WithInv p inv ii pf t1' =>
+    exists t2', p2 = WithInv p inv ii pf t2' /\  
+                     step s1 t1' sc' s2 t2'   
+  | ParStep n sc', ParProc ps =>
+    exists p p' ps1 ps2,
+    [/\ ps = ps1 ++ (n, p) :: ps2,
+     step s1 p sc' s2 p' &
+     p2 = ParProc (ps1 ++ (n, p') :: ps2)]
+  | _, _ => False
+  end.
+
+Fixpoint good (W : world) A (p : proc W A) sc  : Prop :=
+  match sc, p with
+  | ActStep, Act _ _ => True
+  | SeqRet, Seq _ (Ret _) _ => True
+  | SeqStep sc', Seq _ p' _ => good p' sc'
+  | InjectStep sc', Inject _ _ _ p' => good p' sc'
+  | InjectRet, Inject _ _ _ (Ret _) => True
+  | WithInvStep sc', WithInv _ _ _ _ p' => good p' sc'
+  | WithInvRet, WithInv _ _ _ _ (Ret _) => True
+  | ParStep n sc', ParProc ps =>
+    exists p ps1 ps2, ps = ps1 ++ (n, p) :: ps2 /\ good p sc'
+  | _, _ => False
+  end.
+
+(*
+
+[Safety in small-step semantics]
+
+The safety (in order to make the following step) with respect to the
+schedule is defined inductively on the shape of the program and the
+schedule. Omitting the schedule is not a good idea, at it's required
+in order to "sequentialize" the execution of the program
+structure. Once it's dropped, this structure is lost.
+
+ *)
+
+Fixpoint safe (W : world) A (p : proc W A) (this : nid) sc (s : state) : Prop :=
+  match sc, p with
+  | ActStep, Act n a => n == this /\ @a_safe _ _ n a s
+  | SeqRet, Seq _ (Ret _) _ => True
+  | SeqStep sc', Seq _ p' _ => safe p' this sc' s
+  | InjectStep sc', Inject V K pf p' =>
+      exists s', extends pf s s' /\ safe p' this sc' s'
+  | InjectRet, Inject V K pf (Ret _) => exists s', extends pf s s'
+  | WithInvStep sc', WithInv _ _ _ _ p' => safe p' this sc' s
+  | WithInvRet, WithInv _ _ _ _ (Ret _) => True
+  | ParStep n sc', ParProc ps =>
+    (exists! pp, let: (p, ps1, ps2) := pp in ps = ps1 ++ (n, p) :: ps2) /\
+    (forall p ps1 ps2, ps = ps1 ++ (n, p) :: ps2 -> safe p n sc' s)                                          
+  | _, _ => True
+  end.
+
+Definition pstep (W : world) A s1 (p1 : proc W A) this sc s2 p2 := 
+  [/\ s1 \In Coh W, safe p1 this sc s1 & step s1 p1 sc s2 p2].
+
+(* Some sanity lemmas wrt. stepping *)
+
+Lemma pstep_safe (W : world) A s1 (t : proc W A) this sc s2 q : 
+        pstep s1 t this sc s2 q -> safe t this sc s1.
+Proof. by case. Qed.
+
+(*
+
+The following lemma established the operational "progress" property: a
+program, which is safe and also the schedule is appropriate. Together,
+this implies that we can do a step. 
+ *)
+
+Lemma proc_progress W A s (p : proc W A) this sc : 
+        s \In Coh W -> safe p this sc s -> good p sc ->  
+        exists s' (p' : proc W A), pstep s p this sc s' p'.
+Proof.
+move=>C H1 H2; elim: sc W A this s p H2 H1 C=>[||sc IH|sc IH||sc IH||n sc IH]W A this s. 
+- case=>//=n a _/= [E H]; move/a_step_total: (H)=>[s'][r]H'.
+  by exists s', (Ret r); split=>//=; exists r, H.  
+- by case=>//; move=>B p k/=; case: p=>//b _ _; exists s, (k b). 
+- case=>//B p k/=H1 H2 C.
+  case: (IH W B this s p H1 H2 C)=>s'[p'][G1 G2].
+  by exists s', (Seq p' k); split=>//; exists p'. 
+- case=>// V K pf p/=H1 [z][E]H2 C. 
+  case: (E)=>s3[Z] C1 C2.
+  case: (IH V A this z p H1 H2 C1) =>s'[p']H3; case: H3=>S St.
+  exists (s' \+ s3), (Inject pf p'); split=>//; first by exists z.  
+  by subst s; exists z, s', s3, p'. 
+- case=>//V K pf; case=>// v/=_[s'] E C.          
+  by exists s, (Ret v); split=>//=; exists s'.
+- case=>//pr I ii E p/= H1 H2 C.
+  have C' : s \In Coh (mkWorld pr) by subst W; apply: (with_inv_coh C). 
+  case: (IH (mkWorld pr) A this s p H1 H2 C')=>s'[p']H3.
+  exists s', (WithInv pr I ii E p'); split=>//=.
+  by exists p'; split=>//; case: H3. 
+- case=>//pr I ii E; case=>//v/=_ _ C.          
+  by exists s, (Ret v); split=>//=; exists s. 
+case=>//ps/=[p][ps1][ps2][Z]G1; subst ps.
+case=>[[[[p' ps1'] ps2'] G2]]; case: G2=>E1 E; rewrite E1.
+case: (E (p, ps1, ps2) (erefl _))=>Z1 Z2 Z3; subst p' ps1' ps2'; clear E1.
+move/(_ p ps1 ps2 (erefl _))=>S C.
+case: (IH W A n s p G1 S C)=>s'[p']H; exists s', (ParProc (ps1 ++ (n, p') :: ps2)).
+split=>//=; last by exists p, p', ps1, ps2; split=>//; case: H. 
+split; last by move=> x1 x2 x3; case/(E (x1, x2, x3))=><-. 
+by exists (p, ps1, ps2).
+Qed.
+
+(* Some view lemmas for processes and corresponding schedules *)
+
+Lemma stepUnfin W A s1 this sc s2 (t : proc W A) : 
+        pstep s1 Unfinished this sc s2 t <-> False.
+Proof. by split=>//; case; case: sc. Qed.
+
+Lemma stepRet W A s1 this sc s2 (t : proc W A) v : 
+        pstep s1 (Ret v) this sc s2 t <-> False.
+Proof. by split=>//; case; case: sc. Qed.
+
+Lemma stepAct W A s1 this a sc s2 (t : proc W A) : 
+        pstep s1 (Act this a) this sc s2 t <->
+        exists v pf, [/\ sc = ActStep, t = Ret v & @a_step _ _ _ a s1 pf s2 v].
+Proof.
+split; first by case=>C; case: sc=>//= c [v [pf [H ->]]]; exists v, pf. 
+case=>v[pf] [->-> H]; split=>//; last by exists v, pf.
+by apply: (a_safe_coh pf). 
+Qed.
+
+Lemma stepSeq W A B s1 (t : proc W B) k this sc s2 (q : proc W A) :
+        pstep s1 (Seq t k) this sc s2 q <->
+        (exists v, [/\ sc = SeqRet, t = Ret v, q = k v, s2 = s1 &
+                       s1 \In Coh W]) \/
+         exists sc' p',
+           [/\ sc = SeqStep sc', q = Seq p' k & pstep s1 t this sc' s2 p'].
+Proof.
+split; last first.
+- case; first by case=>v [->->->->]. 
+  by case=>sc' [t'][->->][S H]; do !split=>//; exists t'. 
+case; case: sc=>//[|sc] C. 
+- by case: t=>//= v _ [->->]; left; exists v. 
+by move=>G /= [p' [H1 ->]]; right; exists sc, p'.
+Qed.
+
+Lemma stepPar W A s1 ps this sc s2 (q : proc W A) :
+  pstep s1 (ParProc ps) this sc s2 q <->
+  exists n sc',
+    sc = ParStep n sc' /\
+    exists p p' ps1 ps2,
+      [/\ ps = ps1 ++ (n, p) :: ps2,
+       q = ParProc (ps1 ++ (n, p') :: ps2),
+       (exists! pp, let: (p, ps1, ps2) := pp in ps = ps1 ++ (n, p) :: ps2)&
+       pstep s1 p n sc' s2 p'].
+Proof.
+split=>/=; last first.
+- case=>n[s'][->{sc}][p][p'][ps1][ps2][->->{ps q}]U[C] H1 H2.
+  split=>//=; last by exists p, p', ps1, ps2.
+  split=>//; clear H2 p'; case: U=>[[[p' ps1']] ps2'][Z]E.
+  case: (E (p, ps1, ps2) (erefl _))=>Z1 Z2 Z3; subst p' ps2' ps1'.
+  by move=>x1 x2 x3; case/(E (x1, x2, x3))=><-. 
+case; case: sc=>//n sc' C/=G1 G2; exists n, sc'; split=>//.
+case:G1; case=>[[[p ps1]ps2]]U H; case: U=>Z U; subst ps.
+case: G2=>p1[p'][ps1'][ps2'][Z]S->.
+case: (U (p1, ps1', ps2') Z)=>Z1 Z2 Z3. subst p1 ps1' ps2'.
+move: (H _ _ _ Z)=>{H Z}H.
+by exists p, p', ps1, ps2; split=>//; exists (p, ps1, ps2). 
+Qed.
+
+Lemma stepInject V W K A (em : injects V W K) 
+                s1 (t : proc V A) this sc s2 (q : proc W A) :
+  pstep s1 (Inject em t) this sc s2 q <->
+  (* Case 1 : stepped to the final state s1' of the inner program*)
+  (exists s1' v, [/\ sc = InjectRet, t = Ret v, q = Ret v, s2 = s1 &
+                     extends em s1 s1']) \/
+  (* Case 2 : stepped to the nextx state s12 of the inner program*)
+  exists sc' t' s1' s2' s, 
+    [/\ sc = InjectStep sc', q = Inject em t', 
+     s1 = s1' \+ s, s2 = s2' \+ s, s1 \In Coh W &
+              pstep s1' t this sc' s2' t'].
+Proof.
+split; last first.
+- case.
+  + case=>s1' [v][->->->->] E.
+    split=>//=; [by case: E=>x[] | by exists s1'|by exists s1'].
+  case=>sc' [t'][s1'][s2'][s][->->->-> C][[C' S] T]. 
+  split=>//=; last by exists s1', s2', s, t'. 
+  by exists s1'; split=>//; exists s. 
+case=>C; case: sc=>//=; last first.
+- case: t=>//= v [C1 S][s1'][->->{s2 q}] X.
+  by left; exists s1'; exists v. 
+move=>sc /= [s'][X] S [s1'][s2'][t'][t2'][??? C1'] T; subst q s1 s2. 
+right; exists sc, t2', s1', s2', t'; do !split=>//.
+by case: X=>t'' [E] Cs' _; rewrite (coh_prec (cohS C) E _ Cs'). 
+Qed.
+
+Lemma stepWithInv W A pr I (ii : InductiveInv pr I) s1 
+      (t : proc (mkWorld pr) A) this sc s2 (q : proc W A) pf :
+  pstep s1 (WithInv pr I ii pf t) this sc s2 q <-> 
+  (exists v, [/\ sc = WithInvRet, t = Ret v, q = Ret v, s2 = s1,
+                 s1 \In Coh W & W = mkWorld (ProtocolWithIndInv ii)]) \/
+  exists sc' t' , [/\ sc = WithInvStep sc', q = WithInv pr I ii pf t',
+                      W = mkWorld (ProtocolWithIndInv ii),
+                      s1 \In Coh W & pstep s1 t this sc' s2 t'].
+Proof.
+split; last first.
+- case.
+  + by case=>v[->->->->{s2}]C E; split=>//=; exists s1.
+   by case=>sc' [t'][->->{sc q}]E C[C' S]T; split=>//=; exists t'.   
+case=>C; case: sc=>//=; last first.
+- by case: t=>//=v _[s1'][Z1]Z2 Z3; subst s2 s1' q; left; exists v. 
+move=>sc /=S[t'][->{q}T]; right; exists sc, t'; split=>//.
+by split=>//; subst W; apply: (with_inv_coh C).
+Qed.
+
+(*
+
+[Stepping and network semantics]
+
+The following lemma ensures that the operational semantics of our
+programs respect the global network semantics.
+
+ *)
+
+Lemma pstep_network_sem (W : world) A s1 (t : proc W A) this sc s2 q :
+        pstep s1 t this sc s2 q -> network_step W this s1 s2.
+Proof.
+elim: sc W A this s1 s2 t q=>/=.
+- move=>W A this s1 s2 p q; case: p; do?[by case|by move=>?; case| by move=>??; case].
+  + (* move=>n a. *)
+    (* Check (stepAct s1 a ActStep s2 q). *)
+  (* [v][pf][Z1]Z2 H. subst q; apply: (a_step_sem H). *)
+    admit.
+  + by move=>???; case. 
+  + by move=>????; case.
+  by move=>?????; case.   
+- move=>W A this s1 s2 p q; case: p; do?[by case|by move=>?; case| by move=>??; case].
+  + move=>B p p0/stepSeq; case=>[[v][_]??? C|[sc'][p'][]]//.
+    by subst p s2; apply: Idle. 
+  by move=>????/stepInject; case=>[[?][?][?]|[?][?][?][?][?][?]]//.
+  by move=>?????; case.   
+- move=>sc HI W A this s1 s2 p q; case: p; do?[by case|by move=>?; case| by move=>??; case].
+  + move=>B p p0/stepSeq; case=>[[?][?]|[sc'][p'][][]? ?]//.
+    by subst sc' q; apply: HI.
+  by move=>????; case=>? _.
+  by move=>?????; case.   
+- move=>sc HI W A this s1 s2 p q; case: p; do?[by case|by move=>?; case| by move=>??; case].
+  + by move=>B p p0; case. 
+  move=>V K pf p/stepInject; case=>[[?][?][?]|[sc'][t'][s1'][s2'][s][][]????]//. 
+  subst sc' q s1 s2=>C; move/HI=>S; apply: (sem_extend pf)=>//.
+  apply/(cohE pf); exists s2', s; case: (step_coh S)=>C1 C2; split=>//.
+  move/(cohE pf): (C)=>[s1][s2][E]C' H.
+  by move: (coh_prec (cohS C) E C1 C')=>Z; subst s1'; rewrite (joinfK (cohS C) E). 
+  by move=>?????; case.   
+- move=>W A this s1 s2 p q; case: p; do?[by case|by move=>?; case| by move=>??; case].
+  + by move=>???; case.
+  + move=>V K i p; case/stepInject=>[[s1'][v][_]??? X|[?][?][?][?][?][?]]//.
+    by subst p q s2; apply: Idle; split=>//; case: X=>x []. 
+  by move=>?????; case.
+- move=>sc HI W A this s1 s2 p q; case: p;
+          do?[by case|by move=>?; case| by move=>??; case
+              |by move=>???; case|by move=>????; case].
+  move=>pr I ii E p; case/(stepWithInv s1); first by case=>?; case.
+  case=>sc'[t'][][]Z1 Z2 _ C1; subst q sc'.
+  by move/HI=>T; subst W; apply: with_inv_step. 
+- move=>W A this s1 s2 t q; do?[by case|by move=>?; case|by move=>???; case].
+  case=>C; case: t=>//pr I ii E; case=>//=v _[s1'][Z1]Z2 Z3.
+  by subst s1' s2 q; apply: Idle.
+move=>n sc HI W A this s1 s2 p q; case: p=>//;
+do?[by case|by move=>?; case|by move=>???; case|by move=>????; case
+   |by move=>?????; case|by move=>??; case].                                    
+move=>ps/stepPar=>[[m]][sc']; case; case=>Z1 Z2; subst n sc'.
+case=>p[p'][ps1][ps2].
+
+  by case=>p[p'][ps1][ps2][_]_ _; apply: HI.
+Qed.
+
+(*
+
+[Inductive invariants and stepping]
+
+The following lemma is the crux of wrapping into inductive invariants, as 
+it leverages the proof of the fact that each transition preserves the invariant.
+
+*)
+
+Lemma pstep_inv A pr I (ii : InductiveInv pr I) s1 s2 sc
+      (t t' : proc this (mkWorld pr) A):
+  s1 \In Coh (mkWorld (ProtocolWithIndInv ii)) ->
+  pstep s1 t sc s2 t' -> 
+  s2 \In Coh (mkWorld (ProtocolWithIndInv ii)).
+Proof. by move=>C1; case/pstep_network_sem/(with_inv_step C1)/step_coh. Qed.
+
+End ProcessSemantics.
+Inductive schedule :=
+  ActStep | SeqRet | SeqStep of schedule |  
+  InjectStep of schedule | InjectRet |
+  WithInvStep of schedule | WithInvRet |
+  (* Step node number n *)
+  ParStep (n : nid) of schedule.
+
+End ProcessSyntax.
+
+Implicit Arguments Unfinished [W A].
+Implicit Arguments Ret [W A].
+Implicit Arguments Act [W A].
+Implicit Arguments Seq [W A B].
+Implicit Arguments WithInv [W A].
+Implicit Arguments ParProc [W A].
+
+Section ProcessSemantics.
+
+Fixpoint step (W : world) A (s1 : state) (p1 : proc W A)
+         sc (s2 : state) (p2 : proc W A) : Prop :=
+  match sc, p1 with
+  (* Action - make a step *)  
+  | ActStep, Act this a => exists v pf, @a_step _ _ this a s1 pf s2 v /\ p2 = Ret v
+  (* Sequencing - apply a continuation *)  
+  | SeqRet, Seq _ (Ret v) k => s2 = s1 /\ p2 = k v
+  | SeqStep sc', Seq _ p' k1 => 
+    exists p'', step s1 p' sc' s2 p'' /\ p2 = Seq p'' k1
+  (* Injection of a non-reduced term *)
+  | InjectRet, Inject V K pf (Ret v) =>
+     exists s1', [/\ s2 = s1, p2 = Ret v & extends pf s1 s1']
+  | InjectStep sc', Inject V K pf t1' =>
+    exists s1' s2' s t2', 
+    [/\ p2 = Inject pf t2', s1 = s1' \+ s, s2 = s2' \+ s, 
+     s1' \In Coh V & step s1' t1' sc' s2' t2']
+  (* Imposing an inductive invariant on a non-reduced term *)
+  | WithInvRet, WithInv p inv ii pf (Ret v) =>
+     exists s1', [/\ s2 = s1, p2 = Ret v & s1 = s1']
+  | WithInvStep sc', WithInv p inv ii pf t1' =>
+    exists t2', p2 = WithInv p inv ii pf t2' /\  
+                     step s1 t1' sc' s2 t2'   
+  | ParStep n sc', ParProc ps =>
+    exists p p' ps1 ps2,
+    [/\ ps = ps1 ++ (n, p) :: ps2,
+     step s1 p sc' s2 p' &
+     p2 = ParProc (ps1 ++ (n, p') :: ps2)]
+  | _, _ => False
+  end.
+
+Fixpoint good (W : world) A (p : proc W A) sc  : Prop :=
+  match sc, p with
+  | ActStep, Act _ _ => True
+  | SeqRet, Seq _ (Ret _) _ => True
+  | SeqStep sc', Seq _ p' _ => good p' sc'
+  | InjectStep sc', Inject _ _ _ p' => good p' sc'
+  | InjectRet, Inject _ _ _ (Ret _) => True
+  | WithInvStep sc', WithInv _ _ _ _ p' => good p' sc'
+  | WithInvRet, WithInv _ _ _ _ (Ret _) => True
+  | ParStep n sc', ParProc ps =>
+    exists p ps1 ps2, ps = ps1 ++ (n, p) :: ps2 /\ good p sc'
+  | _, _ => False
+  end.
+
+(*
+
+[Safety in small-step semantics]
+
+The safety (in order to make the following step) with respect to the
+schedule is defined inductively on the shape of the program and the
+schedule. Omitting the schedule is not a good idea, at it's required
+in order to "sequentialize" the execution of the program
+structure. Once it's dropped, this structure is lost.
+
+ *)
+
+Fixpoint safe (W : world) A (p : proc W A) (this : nid) sc (s : state) : Prop :=
+  match sc, p with
+  | ActStep, Act n a => n == this /\ @a_safe _ _ n a s
+  | SeqRet, Seq _ (Ret _) _ => True
+  | SeqStep sc', Seq _ p' _ => safe p' this sc' s
+  | InjectStep sc', Inject V K pf p' =>
+      exists s', extends pf s s' /\ safe p' this sc' s'
+  | InjectRet, Inject V K pf (Ret _) => exists s', extends pf s s'
+  | WithInvStep sc', WithInv _ _ _ _ p' => safe p' this sc' s
+  | WithInvRet, WithInv _ _ _ _ (Ret _) => True
+  | ParStep n sc', ParProc ps =>
+    (exists! pp, let: (p, ps1, ps2) := pp in ps = ps1 ++ (n, p) :: ps2) /\
+    (forall p ps1 ps2, ps = ps1 ++ (n, p) :: ps2 -> safe p n sc' s)                                          
+  | _, _ => True
+  end.
+
+Definition pstep (W : world) A s1 (p1 : proc W A) this sc s2 p2 := 
+  [/\ s1 \In Coh W, safe p1 this sc s1 & step s1 p1 sc s2 p2].
+
+(* Some sanity lemmas wrt. stepping *)
+
+Lemma pstep_safe (W : world) A s1 (t : proc W A) this sc s2 q : 
+        pstep s1 t this sc s2 q -> safe t this sc s1.
+Proof. by case. Qed.
+
+(*
+
+The following lemma established the operational "progress" property: a
+program, which is safe and also the schedule is appropriate. Together,
+this implies that we can do a step. 
+ *)
+
+Lemma proc_progress W A s (p : proc W A) this sc : 
+        s \In Coh W -> safe p this sc s -> good p sc ->  
+        exists s' (p' : proc W A), pstep s p this sc s' p'.
+Proof.
+move=>C H1 H2; elim: sc W A this s p H2 H1 C=>[||sc IH|sc IH||sc IH||n sc IH]W A this s. 
+- case=>//=n a _/= [E H]; move/a_step_total: (H)=>[s'][r]H'.
+  by exists s', (Ret r); split=>//=; exists r, H.  
+- by case=>//; move=>B p k/=; case: p=>//b _ _; exists s, (k b). 
+- case=>//B p k/=H1 H2 C.
+  case: (IH W B this s p H1 H2 C)=>s'[p'][G1 G2].
+  by exists s', (Seq p' k); split=>//; exists p'. 
+- case=>// V K pf p/=H1 [z][E]H2 C. 
+  case: (E)=>s3[Z] C1 C2.
+  case: (IH V A this z p H1 H2 C1) =>s'[p']H3; case: H3=>S St.
+  exists (s' \+ s3), (Inject pf p'); split=>//; first by exists z.  
+  by subst s; exists z, s', s3, p'. 
+- case=>//V K pf; case=>// v/=_[s'] E C.          
+  by exists s, (Ret v); split=>//=; exists s'.
+- case=>//pr I ii E p/= H1 H2 C.
+  have C' : s \In Coh (mkWorld pr) by subst W; apply: (with_inv_coh C). 
+  case: (IH (mkWorld pr) A this s p H1 H2 C')=>s'[p']H3.
+  exists s', (WithInv pr I ii E p'); split=>//=.
+  by exists p'; split=>//; case: H3. 
+- case=>//pr I ii E; case=>//v/=_ _ C.          
+  by exists s, (Ret v); split=>//=; exists s. 
+case=>//ps/=[p][ps1][ps2][Z]G1; subst ps.
+case=>[[[[p' ps1'] ps2'] G2]]; case: G2=>E1 E; rewrite E1.
+case: (E (p, ps1, ps2) (erefl _))=>Z1 Z2 Z3; subst p' ps1' ps2'; clear E1.
+move/(_ p ps1 ps2 (erefl _))=>S C.
+case: (IH W A n s p G1 S C)=>s'[p']H; exists s', (ParProc (ps1 ++ (n, p') :: ps2)).
+split=>//=; last by exists p, p', ps1, ps2; split=>//; case: H. 
+split; last by move=> x1 x2 x3; case/(E (x1, x2, x3))=><-. 
+by exists (p, ps1, ps2).
+Qed.
+
+(* Some view lemmas for processes and corresponding schedules *)
+
+Lemma stepUnfin W A s1 this sc s2 (t : proc W A) : 
+        pstep s1 Unfinished this sc s2 t <-> False.
+Proof. by split=>//; case; case: sc. Qed.
+
+Lemma stepRet W A s1 this sc s2 (t : proc W A) v : 
+        pstep s1 (Ret v) this sc s2 t <-> False.
+Proof. by split=>//; case; case: sc. Qed.
+
+Lemma stepAct W A s1 this a sc s2 (t : proc W A) : 
+        pstep s1 (Act this a) this sc s2 t <->
+        exists v pf, [/\ sc = ActStep, t = Ret v & @a_step _ _ _ a s1 pf s2 v].
+Proof.
+split; first by case=>C; case: sc=>//= c [v [pf [H ->]]]; exists v, pf. 
+case=>v[pf] [->-> H]; split=>//; last by exists v, pf.
+by apply: (a_safe_coh pf). 
+Qed.
+
+Lemma stepSeq W A B s1 (t : proc W B) k this sc s2 (q : proc W A) :
+        pstep s1 (Seq t k) this sc s2 q <->
+        (exists v, [/\ sc = SeqRet, t = Ret v, q = k v, s2 = s1 &
+                       s1 \In Coh W]) \/
+         exists sc' p',
+           [/\ sc = SeqStep sc', q = Seq p' k & pstep s1 t this sc' s2 p'].
+Proof.
+split; last first.
+- case; first by case=>v [->->->->]. 
+  by case=>sc' [t'][->->][S H]; do !split=>//; exists t'. 
+case; case: sc=>//[|sc] C. 
+- by case: t=>//= v _ [->->]; left; exists v. 
+by move=>G /= [p' [H1 ->]]; right; exists sc, p'.
+Qed.
+
+Lemma stepPar W A s1 ps this sc s2 (q : proc W A) :
+  pstep s1 (ParProc ps) this sc s2 q <->
+  exists n sc',
+    sc = ParStep n sc' /\
+    exists p p' ps1 ps2,
+      [/\ ps = ps1 ++ (n, p) :: ps2,
+       q = ParProc (ps1 ++ (n, p') :: ps2),
+       (exists! pp, let: (p, ps1, ps2) := pp in ps = ps1 ++ (n, p) :: ps2)&
+       pstep s1 p n sc' s2 p'].
+Proof.
+split=>/=; last first.
+- case=>n[s'][->{sc}][p][p'][ps1][ps2][->->{ps q}]U[C] H1 H2.
+  split=>//=; last by exists p, p', ps1, ps2.
+  split=>//; clear H2 p'; case: U=>[[[p' ps1']] ps2'][Z]E.
+  case: (E (p, ps1, ps2) (erefl _))=>Z1 Z2 Z3; subst p' ps2' ps1'.
+  by move=>x1 x2 x3; case/(E (x1, x2, x3))=><-. 
+case; case: sc=>//n sc' C/=G1 G2; exists n, sc'; split=>//.
+case:G1; case=>[[[p ps1]ps2]]U H; case: U=>Z U; subst ps.
+case: G2=>p1[p'][ps1'][ps2'][Z]S->.
+case: (U (p1, ps1', ps2') Z)=>Z1 Z2 Z3. subst p1 ps1' ps2'.
+move: (H _ _ _ Z)=>{H Z}H.
+by exists p, p', ps1, ps2; split=>//; exists (p, ps1, ps2). 
+Qed.
+
+Lemma stepInject V W K A (em : injects V W K) 
+                s1 (t : proc V A) this sc s2 (q : proc W A) :
+  pstep s1 (Inject em t) this sc s2 q <->
+  (* Case 1 : stepped to the final state s1' of the inner program*)
+  (exists s1' v, [/\ sc = InjectRet, t = Ret v, q = Ret v, s2 = s1 &
+                     extends em s1 s1']) \/
+  (* Case 2 : stepped to the nextx state s12 of the inner program*)
+  exists sc' t' s1' s2' s, 
+    [/\ sc = InjectStep sc', q = Inject em t', 
+     s1 = s1' \+ s, s2 = s2' \+ s, s1 \In Coh W &
+              pstep s1' t this sc' s2' t'].
+Proof.
+split; last first.
+- case.
+  + case=>s1' [v][->->->->] E.
+    split=>//=; [by case: E=>x[] | by exists s1'|by exists s1'].
+  case=>sc' [t'][s1'][s2'][s][->->->-> C][[C' S] T]. 
+  split=>//=; last by exists s1', s2', s, t'. 
+  by exists s1'; split=>//; exists s. 
+case=>C; case: sc=>//=; last first.
+- case: t=>//= v [C1 S][s1'][->->{s2 q}] X.
+  by left; exists s1'; exists v. 
+move=>sc /= [s'][X] S [s1'][s2'][t'][t2'][??? C1'] T; subst q s1 s2. 
+right; exists sc, t2', s1', s2', t'; do !split=>//.
+by case: X=>t'' [E] Cs' _; rewrite (coh_prec (cohS C) E _ Cs'). 
+Qed.
+
+Lemma stepWithInv W A pr I (ii : InductiveInv pr I) s1 
+      (t : proc (mkWorld pr) A) this sc s2 (q : proc W A) pf :
+  pstep s1 (WithInv pr I ii pf t) this sc s2 q <-> 
+  (exists v, [/\ sc = WithInvRet, t = Ret v, q = Ret v, s2 = s1,
+                 s1 \In Coh W & W = mkWorld (ProtocolWithIndInv ii)]) \/
+  exists sc' t' , [/\ sc = WithInvStep sc', q = WithInv pr I ii pf t',
+                      W = mkWorld (ProtocolWithIndInv ii),
+                      s1 \In Coh W & pstep s1 t this sc' s2 t'].
+Proof.
+split; last first.
+- case.
+  + by case=>v[->->->->{s2}]C E; split=>//=; exists s1.
+   by case=>sc' [t'][->->{sc q}]E C[C' S]T; split=>//=; exists t'.   
+case=>C; case: sc=>//=; last first.
+- by case: t=>//=v _[s1'][Z1]Z2 Z3; subst s2 s1' q; left; exists v. 
+move=>sc /=S[t'][->{q}T]; right; exists sc, t'; split=>//.
+by split=>//; subst W; apply: (with_inv_coh C).
+Qed.
+
+(*
+
+[Stepping and network semantics]
+
+The following lemma ensures that the operational semantics of our
+programs respect the global network semantics.
+
+ *)
+
+Lemma pstep_network_sem (W : world) A s1 (t : proc W A) this sc s2 q :
+        pstep s1 t this sc s2 q -> network_step W this s1 s2.
+Proof.
+elim: sc W A this s1 s2 t q=>/=.
+- move=>W A this s1 s2 p q; case: p; do?[by case|by move=>?; case| by move=>??; case].
+  + (* move=>n a. *)
+    (* Check (stepAct s1 a ActStep s2 q). *)
+  (* [v][pf][Z1]Z2 H. subst q; apply: (a_step_sem H). *)
+    admit.
+  + by move=>???; case. 
+  + by move=>????; case.
+  by move=>?????; case.   
+- move=>W A this s1 s2 p q; case: p; do?[by case|by move=>?; case| by move=>??; case].
+  + move=>B p p0/stepSeq; case=>[[v][_]??? C|[sc'][p'][]]//.
+    by subst p s2; apply: Idle. 
+  by move=>????/stepInject; case=>[[?][?][?]|[?][?][?][?][?][?]]//.
+  by move=>?????; case.   
+- move=>sc HI W A this s1 s2 p q; case: p; do?[by case|by move=>?; case| by move=>??; case].
+  + move=>B p p0/stepSeq; case=>[[?][?]|[sc'][p'][][]? ?]//.
+    by subst sc' q; apply: HI.
+  by move=>????; case=>? _.
+  by move=>?????; case.   
+- move=>sc HI W A this s1 s2 p q; case: p; do?[by case|by move=>?; case| by move=>??; case].
+  + by move=>B p p0; case. 
+  move=>V K pf p/stepInject; case=>[[?][?][?]|[sc'][t'][s1'][s2'][s][][]????]//. 
+  subst sc' q s1 s2=>C; move/HI=>S; apply: (sem_extend pf)=>//.
+  apply/(cohE pf); exists s2', s; case: (step_coh S)=>C1 C2; split=>//.
+  move/(cohE pf): (C)=>[s1][s2][E]C' H.
+  by move: (coh_prec (cohS C) E C1 C')=>Z; subst s1'; rewrite (joinfK (cohS C) E). 
+  by move=>?????; case.   
+- move=>W A this s1 s2 p q; case: p; do?[by case|by move=>?; case| by move=>??; case].
+  + by move=>???; case.
+  + move=>V K i p; case/stepInject=>[[s1'][v][_]??? X|[?][?][?][?][?][?]]//.
+    by subst p q s2; apply: Idle; split=>//; case: X=>x []. 
+  by move=>?????; case.
+- move=>sc HI W A this s1 s2 p q; case: p;
+          do?[by case|by move=>?; case| by move=>??; case
+              |by move=>???; case|by move=>????; case].
+  move=>pr I ii E p; case/(stepWithInv s1); first by case=>?; case.
+  case=>sc'[t'][][]Z1 Z2 _ C1; subst q sc'.
+  by move/HI=>T; subst W; apply: with_inv_step. 
+- move=>W A this s1 s2 t q; do?[by case|by move=>?; case|by move=>???; case].
+  case=>C; case: t=>//pr I ii E; case=>//=v _[s1'][Z1]Z2 Z3.
+  by subst s1' s2 q; apply: Idle.
+move=>n sc HI W A this s1 s2 p q; case: p=>//;
+do?[by case|by move=>?; case|by move=>???; case|by move=>????; case
+   |by move=>?????; case|by move=>??; case].                                    
+move=>ps/stepPar=>[[m]][sc']; case; case=>Z1 Z2; subst n sc'.
+case=>p[p'][ps1][ps2].
+
+  by case=>p[p'][ps1][ps2][_]_ _; apply: HI.
+Qed.
+
+(*
+
+[Inductive invariants and stepping]
+
+The following lemma is the crux of wrapping into inductive invariants, as 
+it leverages the proof of the fact that each transition preserves the invariant.
+
+*)
+
+Lemma pstep_inv A pr I (ii : InductiveInv pr I) s1 s2 sc
+      (t t' : proc this (mkWorld pr) A):
+  s1 \In Coh (mkWorld (ProtocolWithIndInv ii)) ->
+  pstep s1 t sc s2 t' -> 
+  s2 \In Coh (mkWorld (ProtocolWithIndInv ii)).
+Proof. by move=>C1; case/pstep_network_sem/(with_inv_step C1)/step_coh. Qed.
+
+End ProcessSemantics.
